finish proof of bool_has_bool_interpretation
this means the definitions of the boolean operations are correct (they
constrain interpretations to interpret them with the desired semantics).
this will be important when showing the axiom of infinity (which depends
on many of these constants) is consistent.

hol-light/stateful/holBoolScript.sml
@@ -32,12 +32,16 @@ val Truth_def = ``Absp p === Absp p``
 val And_def = ``Absp (Absq (Absf (Comb (Comb f p) q) === Absf (Comb (Comb f Truth) Truth)))``
 val Implies_def = ``Absp (Absq (And p q === p))``
 val Forall_def = ``AbsP (P === Absx Truth)``
+val Exists_def = ``AbsP (FAq (Implies (FAx (Implies (Comb P x) q)) q))``
+val Or_def = ``Absp (Absq (FAr (Implies (Implies p r) (Implies (Implies q r) r))))``
+val Falsity_def = ``FAp p``
+val Not_def = ``Absp (Implies p Falsity)``
 val mk_bool_ctxt_def = Define`
   mk_bool_ctxt ctxt =
-    ConstDef "~" (Absp (Implies p Falsity)) ::
-    ConstDef "F" (FAp p) ::
-    ConstDef "\\/" (Absp (Absq (FAr (Implies (Implies p r) (Implies (Implies q r) r))))) ::
-    ConstDef "?" (AbsP (FAq (Implies (FAx (Implies (Comb P x) q)) q))) ::
+    ConstDef "~" ^Not_def ::
+    ConstDef "F" ^Falsity_def ::
+    ConstDef "\\/" ^Or_def ::
+    ConstDef "?" ^Exists_def ::
     ConstDef "!" ^Forall_def ::
     ConstDef "==>" ^Implies_def ::
     ConstDef "/\\" ^And_def ::
@@ -163,20 +167,24 @@ val bool_term_ok = store_thm("bool_term_ok",
 
 open holSemanticsTheory holSemanticsExtraTheory setSpecTheory
 
+val mem = ``mem:'U->'U->bool``
+
+val apply_abstract_matchable = store_thm("apply_abstract_matchable",
+  ``∀f x s t u. x <: s ∧ f x <: t ∧ is_set_theory ^mem ∧ f x = u ⇒ Abstract s t f ' x = u``,
+  metis_tac[apply_abstract])
+
 val bool_sig_instances = store_thm("bool_sig_instances",
   ``is_bool_sig sig ⇒
-    instance sig (i:'U interpretation) "T" Bool = (K (tmaof i "T" (K ARB))) ∧
-    instance sig i "F" Bool = (K (tmaof i "F" (K ARB))) ∧
-    instance sig i "==>" (Fun Bool (Fun Bool Bool)) = (K (tmaof i "==>" (K ARB))) ∧
-    instance sig i "/\\" (Fun Bool (Fun Bool Bool)) = (K (tmaof i "/\\" (K ARB))) ∧
-    instance sig i "\\/" (Fun Bool (Fun Bool Bool)) = (K (tmaof i "\\/" (K ARB))) ∧
-    instance sig i "~" (Fun Bool Bool) = (K (tmaof i "~" (K ARB))) ∧
-    instance sig i "!" (Fun (Fun A Bool) Bool) = (λτ. tmaof i "!" (λx. if x = "A" then τ x else ARB)) ∧
-    instance sig i "?" (Fun (Fun A Bool) Bool) = (λτ. tmaof i "?" (λx. if x = "A" then τ x else ARB))``,
+    instance sig (i:'U interpretation) "T" Bool = (K (tmaof i "T" [])) ∧
+    instance sig i "F" Bool = (K (tmaof i "F" [])) ∧
+    instance sig i "==>" (Fun Bool (Fun Bool Bool)) = (K (tmaof i "==>" [])) ∧
+    instance sig i "/\\" (Fun Bool (Fun Bool Bool)) = (K (tmaof i "/\\" [])) ∧
+    instance sig i "\\/" (Fun Bool (Fun Bool Bool)) = (K (tmaof i "\\/" [])) ∧
+    instance sig i "~" (Fun Bool Bool) = (K (tmaof i "~" [])) ∧
+    instance sig i "!" (Fun (Fun A Bool) Bool) = (λτ. tmaof i "!" [τ "A"]) ∧
+    instance sig i "?" (Fun (Fun A Bool) Bool) = (λτ. tmaof i "?" [τ "A"])``,
   rw[is_bool_sig_def] >> imp_res_tac identity_instance >> rw[FUN_EQ_THM] >>
-  rpt AP_TERM_TAC >> rw[FUN_EQ_THM,tyvars_def])
-
-val mem = ``mem:'U->'U->bool``
+  rpt AP_TERM_TAC >> rw[FUN_EQ_THM,tyvars_def] >> EVAL_TAC)
 
 val _ = Parse.temp_overload_on("Boolrel",
   ``λr.  (Abstract boolset (Funspace boolset boolset)
@@ -186,23 +194,19 @@ val _ = Parse.temp_overload_on("Boolrel",
 val is_bool_interpretation_def = xDefine"is_bool_interpretation"`
   is_bool_interpretation0 ^mem i ⇔
     is_std_interpretation i ∧
-    tmaof i interprets "T" on ∅ as K True ∧
-    tmaof i interprets "/\\" on ∅ as K (Boolrel $/\) ∧
-    tmaof i interprets "==>" on ∅ as K (Boolrel $==>) ∧
-    tmaof i interprets "!" on {"A"} as
-       (λτ. Abstract (Funspace (τ"A") boolset) boolset
-              (λP. Boolean (∀x. x <: (τ"A") ⇒ Holds P x))) ∧
-    tmaof i interprets "?" on {"A"} as
-       (λτ. Abstract (Funspace (τ"A") boolset) boolset
-              (λP. Boolean (∃x. x <: (τ"A") ∧ Holds P x))) ∧
-    tmaof i interprets "\\/" on ∅ as K (Boolrel $\/) ∧
-    tmaof i interprets "F" on ∅ as K False ∧
-    tmaof i interprets "~" on ∅ as K (Abstract boolset boolset (λp. Boolean (p ≠ True)))`
+    tmaof i interprets "T" on [] as K True ∧
+    tmaof i interprets "/\\" on [] as K (Boolrel $/\) ∧
+    tmaof i interprets "==>" on [] as K (Boolrel $==>) ∧
+    tmaof i interprets "!" on ["A"] as
+       (λl. Abstract (Funspace (HD l) boolset) boolset
+              (λP. Boolean (∀x. x <: (HD l) ⇒ Holds P x))) ∧
+    tmaof i interprets "?" on ["A"] as
+       (λl. Abstract (Funspace (HD l) boolset) boolset
+              (λP. Boolean (∃x. x <: (HD l) ∧ Holds P x))) ∧
+    tmaof i interprets "\\/" on [] as K (Boolrel $\/) ∧
+    tmaof i interprets "F" on [] as K False ∧
+    tmaof i interprets "~" on [] as K (Abstract boolset boolset (λp. Boolean (p ≠ True)))`
 val _ = Parse.overload_on("is_bool_interpretation",``is_bool_interpretation0 ^mem``)
-
-val apply_abstract_matchable = store_thm("apply_abstract_matchable",
-  ``∀f x s t u. x <: s ∧ f x <: t ∧ is_set_theory ^mem ∧ f x = u ⇒ Abstract s t f ' x = u``,
-  metis_tac[apply_abstract])
 
 val boolrel_in_funspace = prove(
   ``is_set_theory ^mem ⇒ Boolrel R <: Funspace boolset (Funspace boolset boolset)``,
@@ -215,9 +219,13 @@ fun init_tac q =
   first_x_assum(qspec_then q mp_tac) >>
   discharge_hyps >- (unabbrev_all_tac >> EVAL_TAC) >>
   simp[satisfies_def] >>
-  qspecl_then[`tysof sig`,`tyaof i`]mp_tac (UNDISCH valuation_exists) >>
+  strip_tac >>
+  simp[interprets_def] >>
+  qx_gen_tac`τ`>>strip_tac >>
+  qspecl_then[`tysof sig`,`tyaof i`,`τ`]mp_tac (UNDISCH term_valuation_exists) >>
   discharge_hyps >- fs[is_interpretation_def] >> strip_tac >>
-  disch_then(qspec_then`v`mp_tac) >> simp[] >>
+  first_x_assum(qspec_then`(τ,σ)`mp_tac) >> simp[] >>
+  qabbrev_tac`v = (τ,σ)` >>
   `is_structure sig i v` by fs[is_structure_def] >>
   Q.PAT_ABBREV_TAC`eq = l1 === r1` >>
   `term_ok sig eq` by (
@@ -230,7 +238,45 @@ fun init_tac q =
     simp[termsem_def,typeof_equation,welltyped_equation,EQUATION_HAS_TYPE_BOOL] >>
     simp[bool_sig_instances,interprets_def,combinTheory.K_DEF] >> rw[]
 
-(*
+val apply_abstract_tac = rpt ( (
+    qmatch_abbrev_tac`Abstract AA BB CC ' DD <: EE` >>
+    match_mp_tac (UNDISCH apply_in_rng) >>
+    qexists_tac`AA` >>
+    map_every qunabbrev_tac[`AA`,`BB`,`CC`,`DD`,`EE`] >>
+    rw[boolean_in_boolset]
+    ) ORELSE (
+    match_mp_tac (UNDISCH abstract_in_funspace) >>
+    rw[boolean_in_boolset]
+    ) ORELSE (
+    qmatch_abbrev_tac`Boolrel RR ' BB ' CC <: boolset` >>
+    match_mp_tac (UNDISCH apply_in_rng) >>
+    qexists_tac`boolset` >>
+    map_every qunabbrev_tac[`RR`,`BB`,`CC`] >>
+    rw[boolean_in_boolset]
+    ) ORELSE (
+    qmatch_abbrev_tac`Boolrel RR ' BB <: FF` >>
+    match_mp_tac (UNDISCH apply_in_rng) >>
+    qexists_tac`boolset` >>
+    map_every qunabbrev_tac[`RR`,`BB`,`FF`] >>
+    rw[boolean_in_boolset]
+    )) >>
+    match_mp_tac (UNDISCH apply_in_rng) >>
+    HINT_EXISTS_TAC >> rw[]
+
+val apply_boolrel = prove(
+  ``is_set_theory ^mem ⇒
+    ∀b1 b2. b1 <: boolset ∧ b2 <: boolset ⇒
+      Boolrel R ' b1 ' b2 = Boolean (R (b1 = True) (b2 = True))``,
+  rw[] >>
+  `Boolrel R ' b1 = Abstract boolset boolset (λb2. Boolean (R (b1 = True) (b2 = True)))` by (
+    match_mp_tac apply_abstract_matchable >>
+    rw[] >>
+    match_mp_tac (UNDISCH abstract_in_funspace) >>
+    rw[boolean_in_boolset] ) >>
+  rw[] >>
+  match_mp_tac apply_abstract_matchable >>
+  rw[boolean_in_boolset] )
+
 val bool_has_bool_interpretation = store_thm("bool_has_bool_interpretation",
   ``is_set_theory ^mem ⇒
     ∀ctxt i. theory_ok (thyof (mk_bool_ctxt ctxt)) ∧
@@ -253,26 +299,12 @@ val bool_has_bool_interpretation = store_thm("bool_has_bool_interpretation",
     qpat_assum`is_std_sig sig` mp_tac >>
     simp[is_std_sig_def,Abbr`sig`,Abbr`ctx`]) >>
   conj_asm1_tac >- (
-    fs[models_def] >>
-    first_x_assum(qspec_then`Const "T" Bool === ^Truth_def`mp_tac) >>
-    discharge_hyps >- (unabbrev_all_tac >> EVAL_TAC) >>
-    simp[satisfies_def] >>
-    qspecl_then[`tysof sig`,`tyaof i`]mp_tac (UNDISCH valuation_exists) >>
-    discharge_hyps >- fs[is_interpretation_def] >> strip_tac >>
-    disch_then(qspec_then`v`mp_tac) >> simp[] >>
-    `is_structure sig i v` by fs[is_structure_def] >>
-    `term_ok sig (Truth === Absp p === Absp p)` by (
-      asm_simp_tac (srw_ss()) [term_ok_clauses,typeof_equation,welltyped_equation,EQUATION_HAS_TYPE_BOOL,bool_term_ok] ) >>
+    init_tac`Const "T" Bool === ^Truth_def` >>
     `term_ok sig (Absp p === Absp p)` by (
       simp[term_ok_equation,term_ok_clauses] ) >>
-    rfs[Abbr`sig`,termsem_equation,boolean_eq_true,termsem_def] >>
-    simp[bool_sig_instances,interprets_def] >>
-    rw[combinTheory.K_DEF] >>
-    `τ = λx. ARB` by simp[FUN_EQ_THM] >>
-    simp[boolean_def]) >>
+    rfs[Abbr`sig`,termsem_equation,boolean_eq_true,termsem_def]) >>
   conj_asm1_tac >- (
     init_tac `Const "/\\" (Fun Bool (Fun Bool Bool)) === ^And_def` >>
-    `τ = λx. ARB` by simp[FUN_EQ_THM] >> rw[] >> ntac 2 (pop_assum kall_tac) >>
     imp_res_tac is_std_interpretation_is_type >>
     imp_res_tac typesem_Bool >> simp[] >>
     match_mp_tac (UNDISCH abstract_eq) >>
@@ -310,6 +342,7 @@ val bool_has_bool_interpretation = store_thm("bool_has_bool_interpretation",
     simp[termsem_def] >>
     simp[combinTheory.APPLY_UPDATE_THM,Abbr`vv`] >>
     simp[bool_sig_instances] >> fs[interprets_def] >>
+    last_x_assum(qspec_then`τ`mp_tac)>>simp[]>>strip_tac >>
     rw[boolean_def] >>
     qmatch_assum_abbrev_tac`f1 = f2` >>
     `f1 ' (Boolrel $/\) = False` by (
@@ -337,11 +370,10 @@ val bool_has_bool_interpretation = store_thm("bool_has_bool_interpretation",
         simp[boolean_in_boolset]) >>
       simp[] >>
       match_mp_tac apply_abstract_matchable >>
-    simp[boolean_def,mem_boolset] ) >>
+      simp[boolean_def,mem_boolset] ) >>
     metis_tac[] ) >>
   conj_asm1_tac >- (
     init_tac `Const "==>" (Fun Bool (Fun Bool Bool)) === ^Implies_def` >>
-    `τ = λx. ARB` by simp[FUN_EQ_THM] >> rw[] >> ntac 2 (pop_assum kall_tac) >>
     imp_res_tac is_std_interpretation_is_type >>
     imp_res_tac typesem_Bool >> simp[] >>
     match_mp_tac (UNDISCH abstract_eq) >>
@@ -379,6 +411,7 @@ val bool_has_bool_interpretation = store_thm("bool_has_bool_interpretation",
     simp[termsem_def] >>
     simp[combinTheory.APPLY_UPDATE_THM,Abbr`vv`] >>
     simp[bool_sig_instances] >> fs[interprets_def] >>
+    ntac 2(last_x_assum(qspec_then`τ`mp_tac)>>simp[]>>strip_tac) >>
     `Boolrel $/\ ' b1 = Abstract boolset boolset (λb2. Boolean (b1 = True ∧ b2 = True))` by (
       match_mp_tac apply_abstract_matchable >> simp[] >>
       match_mp_tac (UNDISCH abstract_in_funspace) >> simp[boolean_in_boolset]) >>
@@ -389,17 +422,174 @@ val bool_has_bool_interpretation = store_thm("bool_has_bool_interpretation",
     metis_tac[mem_boolset] ) >>
   conj_asm1_tac >- (
     init_tac `Const "!" (Fun (Fun A Bool) Bool) === ^Forall_def` >>
-    qmatch_assum_abbrev_tac `tmaof i name ff = yy` >>
-    `τ = ff` by (
-      simp[FUN_EQ_THM,Abbr`ff`] >> rw[]
-
-    `τ = λx. ARB` by simp[FUN_EQ_THM] >> rw[] >> ntac 2 (pop_assum kall_tac) >>
+    `τ = tyvof v` by simp[Abbr`v`] >> fs[] >>
+    imp_res_tac is_std_interpretation_is_type >>
+    imp_res_tac typesem_Bool >> simp[] >>
+    imp_res_tac typesem_Fun >> simp[typesem_def] >>
+    match_mp_tac (UNDISCH abstract_eq) >>
+    qx_gen_tac`pp` >> strip_tac >>
+    simp[boolean_in_boolset] >>
+    Q.PAT_ABBREV_TAC`vv = X:'U valuation` >>
+    Q.PAT_ABBREV_TAC`eq = l1 === r1` >>
+    `is_structure sig i vv` by (
+      fs[is_structure_def,Abbr`vv`,is_valuation_def,is_term_valuation_def,combinTheory.APPLY_UPDATE_THM] >>
+      rw[] >> metis_tac[typesem_def] ) >>
+    `term_ok sig eq` by (
+      unabbrev_all_tac >>
+      simp[term_ok_clauses,EQUATION_HAS_TYPE_BOOL,welltyped_equation,typeof_equation,bool_term_ok] ) >>
+    qunabbrev_tac`eq` >>
+    simp[termsem_equation,boolean_in_boolset] >>
+    simp[termsem_def] >>
+    simp[combinTheory.APPLY_UPDATE_THM,Abbr`vv`] >>
+    simp[bool_sig_instances] >> fs[interprets_def] >>
+    ntac 3(last_x_assum(qspec_then`τ`mp_tac)>>simp[]>>strip_tac) >>
+    simp[typesem_def] >>
+    Q.PAT_ABBREV_TAC`aa:'U = X "A"` >>
+    qspecl_then[`pp`,`aa`,`boolset`]mp_tac(UNDISCH in_funspace_abstract) >>
+    discharge_hyps >- (fs[is_type_valuation_def,Abbr`aa`] >> metis_tac[boolean_in_boolset]) >>
+    disch_then(qx_choose_then`pf`strip_assume_tac) >> simp[] >>
+    `∀x. x <: aa ⇒ Abstract aa boolset (λm. True) ' x = True` by (
+      rw[] >> match_mp_tac apply_abstract_matchable >> rw[mem_boolset] ) >>
+    `∀x. x <: aa ⇒ Abstract aa boolset pf ' x = pf x` by (
+      rw[] >> match_mp_tac apply_abstract_matchable >> rw[mem_boolset] ) >>
+    rw[boolean_def,holds_def] >> fs[] >- metis_tac[mem_boolset] >>
+    qmatch_assum_abbrev_tac`f1 ≠ f2` >>
+    qsuff_tac`f1 = f2`>-rw[]>>unabbrev_all_tac >>
+    match_mp_tac (UNDISCH abstract_eq) >>
+    simp[mem_boolset] ) >>
+  conj_asm1_tac >- (
+    init_tac `Const "?" (Fun (Fun A Bool) Bool) === ^Exists_def` >>
+    `τ = tyvof v` by simp[Abbr`v`] >> fs[] >>
+    imp_res_tac is_std_interpretation_is_type >>
+    imp_res_tac typesem_Bool >> simp[] >>
+    imp_res_tac typesem_Fun >> simp[typesem_def] >>
+    match_mp_tac (UNDISCH abstract_eq) >>
+    qx_gen_tac`pp` >> strip_tac >>
+    simp[boolean_in_boolset] >>
+    qspecl_then[`sig`,`i`,`"!"`,`Fun (Fun Bool Bool) Bool`,`Fun (Fun A Bool) Bool`,`[(Bool,A)]`]mp_tac instance_def >>
+    discharge_hyps >- (fs[is_bool_sig_def] >> EVAL_TAC) >>
+    simp[] >> disch_then kall_tac >>
+    simp[tyvars_def,STRING_SORT_def,LIST_UNION_def,LIST_INSERT_def,INORDER_INSERT_def,REV_ASSOCD] >>
+    fs[interprets_def] >>
+    qpat_assum`∀t. is_type_valuation t ⇒ Z`(fn th => assume_tac th >> (qspec_then`("A" =+ boolset)τ`mp_tac) th) >>
+    discharge_hyps >- (
+      fs[is_type_valuation_def,combinTheory.APPLY_UPDATE_THM] >> rw[] >>
+      metis_tac[boolean_in_boolset] ) >>
+    simp[combinTheory.APPLY_UPDATE_THM] >>
+    disch_then kall_tac >>
+    ntac 3(last_x_assum(qspec_then`τ`mp_tac)>>simp[]>>strip_tac) >>
+    first_x_assum(qspec_then`τ`mp_tac)>>simp[]>>strip_tac >>
+    conj_tac >- apply_abstract_tac >>
+    match_mp_tac apply_abstract_matchable >>
+    simp[boolean_in_boolset] >>
+    conj_tac >- apply_abstract_tac >>
+    qmatch_abbrev_tac`Boolean(∀x. x <: boolset ⇒ Holds (Abstract bs bs ff) x) = Z` >>
+    `∀x. x <: boolset ⇒ Abstract bs bs ff ' x = ff x` by (
+      rw[] >>
+      match_mp_tac apply_abstract_matchable >>
+      simp[Abbr`ff`,Abbr`bs`] >>
+      apply_abstract_tac ) >>
+    simp[Abbr`bs`,Abbr`Z`,holds_def] >>
+    simp[Abbr`ff`] >>
+    qho_match_abbrev_tac`Boolean(∀x. x <: boolset ⇒ (Boolrel R ' (Abstract d1 bs i1 ' (Abstract d2 bs (i2 x)))) ' x = True) = Z` >>
+    `∀x. x <: boolset ⇒ Abstract d1 bs i1 ' (Abstract d2 bs (i2 x)) = i1 (Abstract d2 bs (i2 x))` by (
+      rw[] >>
+      match_mp_tac apply_abstract_matchable >>
+      simp[Abbr`bs`,Abbr`d1`,Abbr`i1`,boolean_in_boolset] >>
+      match_mp_tac (UNDISCH abstract_in_funspace) >>
+      rw[Abbr`i2`] >>
+      apply_abstract_tac ) >>
+    simp[Abbr`R`,Abbr`bs`,Abbr`d2`] >>
+    `∀x. (λm. i2 x m) = (i2 x)` by metis_tac[ETA_AX] >>
+    simp[Abbr`i1`] >>
+    simp[holds_def] >>
+    `∀x a. x <: boolset ∧ a <: tyvof v "A" ⇒ Abstract (tyvof v "A") boolset (i2 x) ' a = i2 x a` by (
+      rw[] >>
+      match_mp_tac apply_abstract_matchable >>
+      rw[Abbr`i2`] >>
+      apply_abstract_tac ) >>
+    simp[Abbr`i2`] >>
+    simp[apply_boolrel,boolean_in_boolset,boolean_eq_true,Abbr`Z`] >>
+    `∀x. x <: tyvof v "A" ⇒ pp ' x <: boolset` by (rw[] >> apply_abstract_tac) >>
+    simp[apply_boolrel,boolean_eq_true] >>
+    ntac 20 (pop_assum kall_tac) >>
+    simp[boolean_def] >>
+    metis_tac[mem_boolset] ) >>
+  conj_asm1_tac >- (
+    init_tac `Const "\\/" (Fun Bool (Fun Bool Bool)) === ^Or_def` >>
+    pop_assum kall_tac >>
     imp_res_tac is_std_interpretation_is_type >>
     imp_res_tac typesem_Bool >> simp[] >>
     match_mp_tac (UNDISCH abstract_eq) >>
     imp_res_tac typesem_Fun >>
-*)
-
+    qspecl_then[`sig`,`i`,`"!"`,`Fun (Fun Bool Bool) Bool`,`Fun (Fun A Bool) Bool`,`[(Bool,A)]`]mp_tac instance_def >>
+    discharge_hyps >- (fs[is_bool_sig_def] >> EVAL_TAC) >>
+    simp[] >> disch_then kall_tac >>
+    simp[tyvars_def,STRING_SORT_def,LIST_UNION_def,LIST_INSERT_def,INORDER_INSERT_def,REV_ASSOCD] >>
+    fs[interprets_def] >>
+    qpat_assum`∀t. is_type_valuation t ⇒ tmaof i "!" Z = Y`(fn th => assume_tac th >> (qspec_then`("A" =+ boolset)τ`mp_tac) th) >>
+    discharge_hyps >- (
+      fs[is_type_valuation_def,combinTheory.APPLY_UPDATE_THM] >> rw[] >>
+      metis_tac[boolean_in_boolset] ) >>
+    simp[combinTheory.APPLY_UPDATE_THM] >>
+    disch_then kall_tac >>
+    ntac 3(last_x_assum(qspec_then`τ`mp_tac)>>simp[]>>strip_tac) >>
+    qx_gen_tac`b1` >> strip_tac >> simp[] >>
+    conj_tac >- apply_abstract_tac >>
+    conj_tac >- apply_abstract_tac >>
+    match_mp_tac (UNDISCH abstract_eq) >>
+    qx_gen_tac`b2` >> strip_tac >> simp[] >>
+    simp[boolean_in_boolset] >>
+    conj_tac >- apply_abstract_tac >>
+    match_mp_tac apply_abstract_matchable >>
+    simp[boolean_in_boolset] >>
+    conj_tac >- apply_abstract_tac >>
+    qmatch_abbrev_tac`Boolean (∀x. x <: boolset ⇒ Holds (Abstract boolset boolset ff) x) = Z` >>
+    `∀x. x <: boolset ⇒ Abstract boolset boolset ff ' x = ff x` by (
+      rw[] >>
+      match_mp_tac apply_abstract_matchable >>
+      rw[Abbr`ff`] >>
+      apply_abstract_tac ) >>
+    rw[holds_def] >>
+    simp[apply_boolrel,Abbr`ff`,boolean_in_boolset,Abbr`Z`] >>
+    simp[boolean_def] >>
+    metis_tac[mem_boolset] ) >>
+  conj_asm1_tac >- (
+    init_tac`Const "F" Bool === ^Falsity_def` >>
+    pop_assum kall_tac >>
+    imp_res_tac is_std_interpretation_is_type >>
+    imp_res_tac typesem_Bool >> simp[] >>
+    imp_res_tac typesem_Fun >>
+    qspecl_then[`sig`,`i`,`"!"`,`Fun (Fun Bool Bool) Bool`,`Fun (Fun A Bool) Bool`,`[(Bool,A)]`]mp_tac instance_def >>
+    discharge_hyps >- (fs[is_bool_sig_def] >> EVAL_TAC) >>
+    simp[] >> disch_then kall_tac >>
+    simp[tyvars_def,STRING_SORT_def,LIST_UNION_def,LIST_INSERT_def,INORDER_INSERT_def,REV_ASSOCD] >>
+    fs[interprets_def] >>
+    qpat_assum`∀t. is_type_valuation t ⇒ tmaof i "!" Z = Y`(fn th => assume_tac th >> (qspec_then`("A" =+ boolset)τ`mp_tac) th) >>
+    discharge_hyps >- (
+      fs[is_type_valuation_def,combinTheory.APPLY_UPDATE_THM] >> rw[] >>
+      metis_tac[boolean_in_boolset] ) >>
+    simp[combinTheory.APPLY_UPDATE_THM] >> disch_then kall_tac >>
+    match_mp_tac apply_abstract_matchable >>
+    simp[boolean_in_boolset] >>
+    conj_tac >- (
+      match_mp_tac (UNDISCH abstract_in_funspace) >>
+      rw[] ) >>
+    rw[boolean_def] >>
+    first_x_assum(qspec_then`False`mp_tac) >>
+    rw[mem_boolset,holds_def] >>
+    pop_assum(SUBST1_TAC o SYM) >>
+    match_mp_tac apply_abstract_matchable >>
+    simp[mem_boolset] ) >>
+  init_tac`Const "~" (Fun Bool Bool) === ^Not_def` >>
+  pop_assum kall_tac >>
+  imp_res_tac is_std_interpretation_is_type >>
+  imp_res_tac typesem_Bool >> simp[] >>
+  fs[interprets_def] >>
+  rpt (last_x_assum(qspec_then`τ`mp_tac)>>simp[]>>strip_tac) >>
+  match_mp_tac (UNDISCH abstract_eq) >>
+  simp[boolean_in_boolset,apply_boolrel,combinTheory.APPLY_UPDATE_THM,mem_boolset,boolean_def] >>
+  rw[] >> rw[] >> fs[])
 
 (*
 
